src/ecCoreHiPhl.mli
@@ -8,6 +8,7 @@ open EcLogic
 (* -------------------------------------------------------------------- *)
 val process_phl_form     : ty -> goal -> pformula -> form
 val process_phl_formula  : goal -> pformula -> form
+val process_phl_exp      : bool option -> pexpr -> ty -> goal -> expr
 
 val process_prhl_form    : ty -> goal -> pformula -> form
 val process_prhl_formula : goal -> pformula -> form
