src/ecCorePhl.mli
@@ -1,10 +1,13 @@
 (* -------------------------------------------------------------------- *)
 open EcSymbols
+open EcParsetree
 open EcPath
 open EcTypes
 open EcMemory
 open EcModules
 open EcFol
+open EcMetaProg.Zipper
+open EcEnv
 open EcBaseLogic
 open EcLogic
 
@@ -49,7 +52,32 @@ val t_as_equivF   : form -> equivF
 val t_as_equivS   : form -> equivS
 
 (* -------------------------------------------------------------------- *)
+val get_pre  : form -> form
+val get_post : form -> form
+val set_pre  : pre:form -> form -> form
+
+(* -------------------------------------------------------------------- *)
 val t_hS_or_bhS_or_eS : ?th:tactic -> ?tbh:tactic -> ?te:tactic -> tactic
+val t_hF_or_bhF_or_eF : ?th:tactic -> ?tbh:tactic -> ?te:tactic -> tactic
+
+(* -------------------------------------------------------------------- *)
+type 'a code_tx_t =
+     LDecl.hyps -> 'a -> form * form -> memenv * stmt
+  -> memenv * stmt * form list
+
+type zip_t = 
+     LDecl.hyps -> form * form -> memenv -> zipper
+  -> memenv * zipper * form list
+
+val t_zip : zip_t -> codepos code_tx_t
+
+val t_fold : (LDecl.hyps, memenv) folder -> codepos code_tx_t
+
+val t_code_transform :
+      bool option -> ?bdhoare:bool -> 'state
+  -> (bool option -> EcBaseLogic.rule)
+  -> 'state code_tx_t
+  -> tactic
 
 (* -------------------------------------------------------------------- *)
 val s_split_i : string -> int -> stmt -> instr list * instr * instr list
@@ -61,6 +89,9 @@ val id_of_pv : prog_var -> memory -> EcIdent.t
 val id_of_mp : mpath    -> memory -> EcIdent.t
 
 (* -------------------------------------------------------------------- *)
+val fresh_pv : memenv -> variable -> memenv * symbol
+
+(* -------------------------------------------------------------------- *)
 type lv_subst_t = (lpattern * form) * (prog_var * memory * form) list
 
 val mk_let_of_lv_substs : EcEnv.env -> (lv_subst_t list * form) -> form
@@ -68,3 +99,19 @@ val mk_let_of_lv_substs : EcEnv.env -> (lv_subst_t list * form) -> form
 val lv_subst : memory -> lvalue -> form -> lv_subst_t
 
 val subst_form_lv : EcEnv.env -> memory -> lvalue -> form -> form -> form
+
+(* -------------------------------------------------------------------- *)
+type ai_t = mpath * xpath * oracle_info * funsig
+
+val abstract_info  : EcEnv.env -> xpath -> ai_t
+val abstract_info2 : EcEnv.env -> xpath -> xpath -> ai_t * ai_t
+
+(* -------------------------------------------------------------------- *)
+val mk_inv_spec : EcEnv.env -> form -> xpath -> xpath -> form
+
+(* -------------------------------------------------------------------- *)
+val generalize_subst :
+     EcEnv.env -> memory -> (prog_var * ty) list -> mpath list
+  -> (EcIdent.t * gty) list * (form, form) EcPV.Mpv.t
+
+val generalize_mod : EcEnv.env -> EcIdent.t -> EcPV.PV.t -> form -> form
