src/phl/ecPhlCase.mli
@@ -1,0 +1,20 @@
+(* -------------------------------------------------------------------- *)
+open EcTypes
+open EcFol
+open EcBaseLogic
+open EcLogic
+
+(* -------------------------------------------------------------------- *)
+class rn_hl_case : form ->
+object
+  inherit xrule
+
+  method phi : form
+end
+
+(* -------------------------------------------------------------------- *)
+val t_hoare_case   : form -> tactic
+val t_bdHoare_case : form -> tactic
+val t_equiv_case   : form -> tactic
+
+val t_hl_case : form -> tactic
