src/phl/ecPhlExists.ml
@@ -1,0 +1,93 @@
+(* -------------------------------------------------------------------- *)
+open EcUtils
+open EcFol
+open EcEnv
+open EcBaseLogic
+open EcLogic
+open EcCorePhl
+open EcCoreHiLogic
+
+(* -------------------------------------------------------------------- *)
+class rn_hl_exists_elim = object
+  inherit xrule "[hl] elim-exists"
+end
+
+let rn_hl_exists_elim = RN_xtd (new rn_hl_exists_elim :> xrule)
+
+(* -------------------------------------------------------------------- *)
+module LowInternal = struct
+  let get_to_gen side f = 
+    let do_side m = 
+      match side with
+      | true  when EcIdent.id_equal m mleft  -> true
+      | true  when EcIdent.id_equal m mright -> false
+      | false when EcIdent.id_equal m mhr    -> true
+      | _ -> assert false
+    in
+      match f.f_node with
+      | Fpvar(pv, m) -> 
+          let id = id_of_pv pv m in
+            (id, do_side m, f_pvar pv f.f_ty, f)
+
+      | Fglob(mp, m) ->
+          let id = id_of_mp mp m in
+            (id, do_side m, f_glob mp, f)
+
+      | _ -> tacuerror "global memory or variable expected"
+
+  let get_to_gens side fs = 
+    List.map (get_to_gen side) fs
+end
+
+(* -------------------------------------------------------------------- *)
+let t_hr_exists_elim g = 
+  let concl = get_concl g in
+  let pre = get_pre concl in
+  let bd, pre = destr_exists pre in
+  (* TODO check that bd is not bind in the post *)
+  let concl = f_forall bd (set_pre ~pre concl) in
+    prove_goal_by [concl] rn_hl_exists_elim g
+
+let t_hr_exists_intro fs g = 
+  let hyps, concl = get_goal g in 
+  let pre = get_pre concl in
+  let post = get_post concl in
+  let side = is_equivS concl || is_equivF concl in
+  let gen = LowInternal.get_to_gens side fs in
+  let eqs = List.map (fun (id,_,_,f) -> f_eq (f_local id f.f_ty) f) gen in
+  let bd = List.map (fun (id,_,_,f) -> id, GTty f.f_ty) gen in
+  let pre = f_exists bd (f_and (f_ands eqs) pre) in
+  let ms = 
+    if   side
+    then LDecl.fresh_ids hyps ["&ml";"&mr";"H"] 
+    else LDecl.fresh_ids hyps ["&m";"H"] in
+  let h = List.hd (List.rev ms) in
+  let args = 
+    let ml = List.hd ms in
+    let mr = if side then List.hd (List.tl ms) else ml in
+    let do1 (_, side, mk, _) = AAform (mk (if side then ml else mr)) in
+      List.map do1 gen
+  in
+    t_seq_subgoal (EcPhlConseq.t_conseq pre post)
+      [t_lseq [t_intros_i ms;
+               gen_t_exists (fun _ _ f -> f) args; 
+               t_hyp h];
+       t_trivial; t_id None]
+      g
+
+(* -------------------------------------------------------------------- *)
+let process_exists_intro fs g = 
+  let hyps,concl = get_goal g in
+  let penv = 
+    match concl.f_node with
+    | FhoareF hf -> fst (LDecl.hoareF hf.hf_f hyps)
+    | FhoareS hs -> LDecl.push_active hs.hs_m hyps 
+    | FbdHoareF bhf ->fst (LDecl.hoareF bhf.bhf_f hyps) 
+    | FbdHoareS bhs -> LDecl.push_active bhs.bhs_m hyps 
+    | FequivF ef -> fst (LDecl.equivF ef.ef_fl ef.ef_fr hyps)
+    | FequivS es -> LDecl.push_all [es.es_ml; es.es_mr] hyps 
+    | _ -> tacuerror "cannot apply conseq rule, not a phl/prhl judgement"
+  in
+
+  let fs = List.map (fun f -> process_form_opt penv f None) fs in
+    t_hr_exists_intro fs g 
