src/phl/ecPhlExists.mli
@@ -1,0 +1,17 @@
+(* -------------------------------------------------------------------- *)
+open EcParsetree
+open EcFol
+open EcBaseLogic
+open EcLogic
+
+(* -------------------------------------------------------------------- *)
+class rn_hl_exists_elim : object
+  inherit xrule
+end
+
+(* -------------------------------------------------------------------- *)
+val t_hr_exists_elim  : tactic
+val t_hr_exists_intro : form list -> tactic
+
+(* -------------------------------------------------------------------- *)
+val process_exists_intro : pformula list -> tactic
