src/phl/ecPhlFel.mli
@@ -1,0 +1,34 @@
+(* -------------------------------------------------------------------- *)
+open EcUtils
+open EcPath
+open EcParsetree
+open EcFol
+open EcBaseLogic
+open EcLogic
+
+(* -------------------------------------------------------------------- *)
+class rn_hl_fel : form -> form -> form -> form -> (xpath * form) list ->
+object
+  inherit xrule
+
+  method ash    : form
+  method cntr   : form
+  method fevent : form
+  method preds  : (xpath * form) list
+  method q      : form
+end
+
+(* -------------------------------------------------------------------- *)
+val t_failure_event :
+  int -> form -> form -> form -> form -> (xpath * form) list -> form -> tactic
+
+(* -------------------------------------------------------------------- *)
+type pfel_t =
+    pformula
+  * pformula
+  * pformula
+  * pformula
+  * (pgamepath * pformula) list
+  * pformula option
+
+val process_fel : int -> pfel_t -> tactic
