src/phl/ecPhlFun.mli
@@ -1,0 +1,62 @@
+(* -------------------------------------------------------------------- *)
+open EcUtils
+open EcParsetree
+open EcTypes
+open EcFol
+open EcBaseLogic
+open EcLogic
+
+(* -------------------------------------------------------------------- *)
+class rn_hl_fun_def : object
+  inherit xrule
+end
+
+class rn_hl_fun_abs : form -> object
+  inherit xrule
+
+  method phi : form
+end
+
+class rn_hl_fun_code : object
+  inherit xrule
+end
+
+class rn_hl_fun_upto : form -> form -> form -> object
+  inherit xrule
+
+  method bad  : form
+  method inv1 : form
+  method inv2 : form
+end
+
+(* -------------------------------------------------------------------- *)
+module FunDefLow : sig
+  val t_hoareF_fun_def   : tactic
+  val t_bdHoareF_fun_def : tactic
+  val t_equivF_fun_def   : tactic
+end
+
+(* -------------------------------------------------------------------- *)
+module FunAbsLow : sig
+  val t_hoareF_abs   : form -> tactic
+  val t_bdHoareF_abs : form -> tactic
+  val t_equivF_abs   : form -> tactic
+end
+
+(* -------------------------------------------------------------------- *)
+module UpToLow : sig
+  val t_equivF_abs_upto : form -> form -> form -> tactic
+end
+
+val t_fun_def : tactic
+val t_fun : form -> tactic
+val t_fun_to_code : tactic
+
+(* -------------------------------------------------------------------- *)
+val process_fun_abs : pformula -> tactic
+
+type p_upto_info = pformula * pformula * (pformula option)
+
+val process_fun_upto_info : p_upto_info -> goal -> form tuple3
+
+val process_fun_upto : p_upto_info -> tactic
