src/phl/ecPhlLoopTx.ml
@@ -1,0 +1,223 @@
+(* -------------------------------------------------------------------- *)
+open EcUtils
+open EcParsetree
+open EcTypes
+open EcModules
+open EcFol
+open EcEnv
+open EcBaseLogic
+open EcLogic
+open EcPV
+open EcMetaProg
+open EcCorePhl
+open EcCoreHiPhl
+
+module Zpr = EcMetaProg.Zipper
+
+(* -------------------------------------------------------------------- *)
+let check_fission_independence env b init c1 c2 c3 =
+  (* TODO improve error message, see swap *)
+  let check_disjoint s1 s2 = 
+    if not (PV.indep env s1 s2) then
+      tacuerror "in loop-fission, independence check failed"
+  in
+
+  let fv_b    = e_read   env PV.empty b    in
+  let rd_init = is_read  env PV.empty init in
+  let wr_init = is_write env PV.empty init in
+  let rd_c1   = is_read  env PV.empty c1   in
+  let rd_c2   = is_read  env PV.empty c2   in
+  let rd_c3   = is_read  env PV.empty c3   in
+  let wr_c1   = is_write env PV.empty c1   in
+  let wr_c2   = is_write env PV.empty c2   in
+  let wr_c3   = is_write env PV.empty c3   in
+
+  check_disjoint rd_c1 wr_c2;
+  check_disjoint rd_c2 wr_c1;
+  List.iter (check_disjoint fv_b) [wr_c1; wr_c2];
+  check_disjoint fv_b (PV.diff wr_c3 wr_init);
+  List.iter (check_disjoint rd_init) [wr_init; wr_c1; wr_c3];
+  List.iter (check_disjoint rd_c3) [wr_c1; wr_c2]
+
+(* -------------------------------------------------------------------- *)
+type fission_t = bool option * codepos * (int * (int * int))
+
+class rn_hl_fission side pos split =
+object
+  inherit xrule "[hl] loop-fission"
+
+  method side     : bool option       = side
+  method position : codepos           = pos
+  method split    : int * (int * int) = split
+end
+
+let rn_hl_fission side pos split =
+  RN_xtd (new rn_hl_fission side pos split :> xrule)
+
+let fission_stmt (il, (d1, d2)) env me zpr =
+  if d2 < d1 then
+    tacuerror "%s, %s"
+      "in loop-fission"
+      "second break offset must not be lower than the first one";
+  
+  let (hd, init, b, sw, tl) =
+    match zpr.Zpr.z_tail with
+    | { i_node = Swhile (b, sw) } :: tl -> begin
+        if List.length zpr.Zpr.z_head < il then
+          tacuerror "while-loop is not headed by %d intructions" il;
+      let (init, hd) = List.take_n il zpr.Zpr.z_head in
+        (hd, init, b, sw, tl)
+      end
+    | _ -> tacuerror "code position does not lead to a while-loop"
+  in
+
+  if d2 > List.length sw.s_node then
+    tacuerror "in loop fission, invalid offsets range";
+
+  let (s1, s2, s3) =
+    let (s1, s2) = List.take_n (d1   ) sw.s_node in
+    let (s2, s3) = List.take_n (d2-d1) s2 in
+      (s1, s2, s3)
+  in
+
+  check_fission_independence env b init s1 s2 s3;
+
+  let wl1 = i_while (b, stmt (s1 @ s3)) in
+  let wl2 = i_while (b, stmt (s2 @ s3)) in
+  let fis =   (List.rev_append init [wl1])
+            @ (List.rev_append init [wl2]) in
+
+    (me, { zpr with Zpr.z_head = hd; Zpr.z_tail = fis @ tl }, [])
+
+let t_fission side cpos infos g =
+  let tr = fun side -> rn_hl_fission side cpos infos in
+  let cb = fun hyps _ me zpr -> fission_stmt infos (LDecl.toenv hyps) me zpr in
+    t_code_transform side cpos tr (t_zip cb) g
+
+let process_fission (side, cpos, infos) g =
+  t_fission side cpos infos g
+
+(* -------------------------------------------------------------------- *)
+type fusion_t = bool option * codepos * (int * (int * int))
+
+class rn_hl_fusion side pos split =
+object
+  inherit xrule "[hl] loop-fusion"
+
+  method side     : bool option       = side
+  method position : codepos           = pos
+  method split    : int * (int * int) = split
+end
+
+let rn_hl_fusion side pos split =
+  RN_xtd (new rn_hl_fusion side pos split :> xrule)
+
+let fusion_stmt (il, (d1, d2)) env me zpr =
+  let (hd, init1, b1, sw1, tl) =
+    match zpr.Zpr.z_tail with
+    | { i_node = Swhile (b, sw) } :: tl -> begin
+        if List.length zpr.Zpr.z_head < il then
+          tacuerror "1st while-loop is not headed by %d intruction(s)" il;
+      let (init, hd) = List.take_n il zpr.Zpr.z_head in
+        (hd, init, b, sw, tl)
+      end
+    | _ -> tacuerror "code position does not lead to a while-loop"
+  in
+
+  let (init2, b2, sw2, tl) =
+    if List.length tl < il then
+      tacuerror "1st first-loop is not followed by %d instruction(s)" il;
+    let (init2, tl) = List.take_n il tl in
+      match tl with
+      | { i_node = Swhile (b2, sw2) } :: tl -> (List.rev init2, b2, sw2, tl)
+      | _ -> tacuerror "cannot find the 2nd while-loop"
+  in
+
+  if d1 > List.length sw1.s_node then
+    tacuerror "in loop-fusion, body is less than %d instruction(s)" d1;
+  if d2 > List.length sw2.s_node then
+    tacuerror "in loop-fusion, body is less than %d instruction(s)" d2;
+
+  let (sw1, fini1) = List.take_n d1 sw1.s_node in
+  let (sw2, fini2) = List.take_n d2 sw2.s_node in
+
+  (* FIXME: costly *)
+  if not (EcReduction.s_equal_norm env (stmt init1) (stmt init2)) then
+    tacuerror "in loop-fusion, preludes do not match";
+  if not (EcReduction.s_equal_norm env (stmt fini1) (stmt fini2)) then
+    tacuerror "in loop-fusion, finalizers do not match";
+  if not (EcReduction.e_equal_norm env b1 b2) then
+    tacuerror "in loop-fusion, while conditions do not match";
+
+  check_fission_independence env b1 init1 sw1 sw2 fini1;
+
+  let wl  = i_while (b1, stmt (sw1 @ sw2 @ fini1)) in
+  let fus = List.rev_append init1 [wl] in
+
+    (me, { zpr with Zpr.z_head = hd; Zpr.z_tail = fus @ tl; }, [])
+
+let t_fusion side cpos infos g =
+  let tr = fun side -> rn_hl_fusion side cpos infos in
+  let cb = fun hyps _ me zpr -> fusion_stmt infos (LDecl.toenv hyps) me zpr in
+    t_code_transform side cpos tr (t_zip cb) g
+
+let process_fusion (side, cpos, infos) g =
+  t_fusion side cpos infos g
+
+(* -------------------------------------------------------------------- *)
+type unroll_t = bool option * EcParsetree.codepos
+
+class rn_hl_unroll side pos =
+object
+  inherit xrule "[hl] loop-unroll"
+
+  method side     : bool option = side
+  method position : codepos     = pos
+end
+
+let rn_hl_unroll side pos =
+  RN_xtd (new rn_hl_unroll side pos :> xrule)
+
+let unroll_stmt _ me i =
+  match i.i_node with
+  | Swhile (e, sw) -> (me, [i_if (e, sw, stmt []); i])
+  | _ -> tacuerror "cannot find a while loop at given position"
+
+let t_unroll side cpos g =
+  let tr = fun side -> rn_hl_unroll side cpos in
+    t_code_transform side cpos tr (t_fold unroll_stmt) g
+
+let process_unroll (side, cpos) g =
+  t_unroll side cpos g
+
+(* -------------------------------------------------------------------- *)
+type splitwhile_t = pexpr * bool option * codepos
+
+class rn_hl_splitwhile cond side pos =
+object
+  inherit xrule "[hl] split-while"
+
+  method condition : expr        = cond
+  method side      : bool option = side
+  method position  : codepos     = pos
+end
+
+let rn_hl_splitwhile cond side pos =
+  RN_xtd (new rn_hl_splitwhile cond side pos :> xrule)
+
+let splitwhile_stmt b _env me i =
+  match i.i_node with
+  | Swhile (e, sw) -> 
+      let op_and = e_op EcCoreLib.p_and [] (tfun tbool (tfun tbool tbool)) in
+      let e = e_app op_and [e; b] tbool in
+        (me, [i_while (e, sw); i])
+
+  | _ -> tacuerror "cannot find a while loop at given position"
+
+let t_splitwhile b side cpos g =
+  let tr = fun side -> rn_hl_splitwhile b side cpos in
+    t_code_transform side cpos tr (t_fold (splitwhile_stmt b)) g
+
+let process_splitwhile (b, side, cpos) g =
+  let b = process_phl_exp side b tbool g in
+    t_splitwhile b side cpos g
