src/phl/ecPhlRCond.mli
@@ -1,0 +1,23 @@
+(* -------------------------------------------------------------------- *)
+open EcBaseLogic
+open EcLogic
+
+(* -------------------------------------------------------------------- *)
+class rn_hl_rcond : bool option -> bool -> int ->
+object
+  inherit xrule
+
+  method branch   : bool
+  method position : int
+  method side     : bool option
+end
+
+(* -------------------------------------------------------------------- *)
+module Low : sig
+  val t_hoare_rcond   : bool -> int -> tactic
+  val t_bdHoare_rcond : bool -> int -> tactic
+  val t_equiv_rcond   : bool -> bool -> int -> tactic
+end
+
+(* -------------------------------------------------------------------- *)
+val t_rcond : bool option -> bool -> int -> tactic
