src/phl/ecPhlSp.ml
@@ -1,0 +1,105 @@
+(* -------------------------------------------------------------------- *)
+open EcUtils
+open EcModules
+open EcFol
+open EcBaseLogic
+open EcLogic
+open EcCorePhl
+
+(* -------------------------------------------------------------------- *)
+class rn_hl_sp = object
+  inherit xrule "[hl] SP"
+end
+
+let rn_hl_sp = RN_xtd (new rn_hl_sp :> xrule)
+
+(* -------------------------------------------------------------------- *)
+let rec sp_st side env mem pre (st : stmt) =
+  List.fold_left
+    (fun r i -> sp_inst side env mem r i.i_node)
+    pre st.s_node
+
+and sp_inst side env mem (pre : form) (inst : instr_node) : form =
+  match inst with
+  | Sasgn (LvVar (lf, lty) as lvL, muL) ->
+      let fl   = f_pvar lf lty side in
+      let x_id =
+        if   EcIdent.id_equal mleft side
+        then EcIdent.create (symbol_of_lv lvL ^ "L")
+        else EcIdent.create (symbol_of_lv lvL ^ "R") in
+      let x    = f_local x_id lty in
+      let muL  = EcFol.form_of_expr (EcMemory.memory mem) muL in
+      let muL' = (subst_form_lv env (EcMemory.memory mem) lvL x muL) in
+      let fvl  = EcPV.PV.fv env (EcMemory.memory mem) pre in (* FV(pre) *)
+      let fvm  = EcPV.PV.fv env (EcMemory.memory mem) muL in (* FV(e) *)
+      if (EcPV.PV.mem_pv env lf fvl) || (EcPV.PV.mem_pv env lf fvm) then
+        let pr = subst_form_lv env (EcMemory.memory mem) lvL x pre in
+          f_exists [(x_id, GTty lty)] (f_and_simpl (f_eq fl muL') pr)
+      else
+        f_and_simpl (f_eq fl muL) pre
+
+  | Sif (e, st1, st2) ->
+      let b   = EcFol.form_of_expr (EcMemory.memory mem) e in
+      let pb  = f_and_simpl pre b in
+      let pnb = f_and_simpl pre (f_not b) in
+      let sp1 = sp_st side env mem pb st1 in
+      let sp2 = sp_st side env mem pnb st2 in
+        f_or sp1 sp2
+
+  | _ -> cannot_apply "sp" "instr. is not a single assignment or a conditional"
+
+(* -------------------------------------------------------------------- *)
+let t_sp_aux side g =
+  let (env, _, concl) = get_goal_e g in
+  let (stmt, m, menv, pre, prove_goal) =
+    match concl.f_node with
+    | FequivS es -> begin
+        match side with
+        | true ->
+            let f pr st =
+              let wes = f_equivS_r {es with es_sl=st; es_pr=pr} in
+                t_on_last t_simplify_nodelta (prove_goal_by [wes] rn_hl_sp g)
+            in
+              (es.es_sl,mleft, es.es_ml, es.es_pr, f)
+
+        | false ->
+            let f pr st =
+              let wes = f_equivS_r {es with es_sr=st; es_pr=pr} in
+                t_on_last t_simplify_nodelta (prove_goal_by [wes] rn_hl_sp g)
+            in
+              (es.es_sr, mright, es.es_mr, es.es_pr, f)
+    end
+
+    | FhoareS hs ->
+        let f pr st =
+          let wes = f_hoareS_r {hs with hs_s=st; hs_pr=pr} in
+            t_on_last t_simplify_nodelta (prove_goal_by [wes] rn_hl_sp g)
+        in
+          (hs.hs_s, mhr, hs.hs_m, hs.hs_pr, f)
+
+    | FbdHoareS bhs ->
+        let f pr st =
+          let wes = f_bdHoareS_r {bhs with bhs_s=st; bhs_pr=pr} in
+            t_on_last t_simplify_nodelta (prove_goal_by [wes] rn_hl_sp g)
+        in
+          (bhs.bhs_s, mhr, bhs.bhs_m, bhs.bhs_pr, f)
+
+    | _ -> tacerror (NotPhl None)
+
+  in let (pr, stmt) =
+    let (l, ls) =
+      match stmt.s_node with
+      | []   -> cannot_apply "sp" "statement is empty"
+      | i::s -> (i, EcModules.stmt s)
+    in
+    let pr  = sp_inst m env menv pre l.i_node in
+      (pr, ls)
+  in
+    prove_goal pr stmt
+
+(* -------------------------------------------------------------------- *)
+let t_sp side g =
+  let sp s = t_repeat (t_sp_aux s) in
+    match side with
+    | None   -> t_on_last (sp false) (sp true g)
+    | Some s -> t_repeat  (t_sp_aux s) g
